Verifying and tests passing!

src/StandardLibrary/Consumers.dfy
@@ -7,44 +7,58 @@ module Consumers {
 
   trait ByteConsumer {
     ghost const Repr: set<object>
-    predicate Valid() reads this, Repr ensures Valid() ==> this in Repr
+    predicate Valid() reads this, Repr ensures Valid() ==> this in Repr decreases this, Repr
     predicate method CanAccept() reads this, Repr
       requires Valid()
       ensures Valid()
     method Accept(b: uint8)
       requires Valid()
       requires CanAccept()
-      ensures Valid()
       modifies this, Repr
       decreases Repr
+      ensures Valid()
+      ensures Repr == old(Repr)
   }
 
   trait {:extern} ExternalByteConsumer {
     ghost const Repr: set<object>
+    predicate Valid() reads this, Repr ensures Valid() ==> this in Repr decreases this, Repr
     predicate method CanAccept() reads this, Repr decreases Repr
-    method Accept(b: uint8) modifies this, Repr decreases Repr
+    method Accept(b: uint8) 
+      modifies this, Repr 
+      decreases Repr 
+      ensures Valid()
+      ensures Repr == old(Repr)
   }
 
   class AsExternalByteConsumer extends ExternalByteConsumer {
     const wrapped: ByteConsumer
-    constructor(wrapped: ByteConsumer) {
+    constructor(wrapped: ByteConsumer) 
+      requires wrapped.Valid() 
+      ensures Valid() 
+      ensures this.Repr == {this, wrapped} + wrapped.Repr
+    {
       this.wrapped := wrapped;
       this.Repr := {this, wrapped} + wrapped.Repr;
     }
-    predicate Valid() reads this, Repr ensures Valid() ==> this in Repr {
+    predicate Valid() reads this, Repr ensures Valid() ==> this in Repr decreases this, Repr {
       && this in Repr 
       && wrapped in Repr 
       && wrapped.Repr < Repr 
       && this !in wrapped.Repr
       && wrapped.Valid()
     }
-    lemma {:axiom} AssumedValid() ensures Valid()
     predicate method CanAccept() reads this, Repr decreases Repr {
-      AssumedValid();
+      Axiom(Valid());
       wrapped.CanAccept()
     }
-    method Accept(b: uint8) modifies this, Repr decreases Repr {
-      AssumedValid();
+    method Accept(b: uint8) 
+      modifies this, Repr 
+      decreases Repr 
+      ensures Valid()
+      ensures Repr == old(Repr)
+    {
+      Axiom(Valid());
       expect CanAccept();
       wrapped.Accept(b);
     }
@@ -52,15 +66,19 @@ module Consumers {
 
   class AsByteConsumer extends ByteConsumer {
     const wrapped: ExternalByteConsumer
-    constructor(wrapped: ExternalByteConsumer) ensures Valid() {
+    constructor(wrapped: ExternalByteConsumer) requires wrapped.Valid()
+      ensures Valid()
+      ensures this.Repr == {this, wrapped} + wrapped.Repr
+    {
       this.wrapped := wrapped;
       this.Repr := {this, wrapped} + wrapped.Repr;
     }
-    predicate Valid() reads this, Repr ensures Valid() ==> this in Repr {
+    predicate Valid() reads this, Repr ensures Valid() ==> this in Repr decreases this, Repr {
       && this in Repr 
       && wrapped in Repr 
       && wrapped.Repr < Repr 
       && this !in wrapped.Repr
+      && wrapped.Valid()
     }
     predicate method CanAccept() reads this, Repr
       requires Valid()
@@ -71,19 +89,25 @@ module Consumers {
     }
     method Accept(b: uint8) 
       requires Valid()
-      ensures Valid()
       modifies this, Repr
       decreases Repr
+      ensures Valid()
+      ensures Repr == old(Repr)
     {
       wrapped.Accept(b);
     }
   }
 
   method ToExternalByteConsumer(c: ByteConsumer) returns (res: ExternalByteConsumer)
+    requires c.Valid()
+    ensures res.Valid()
+    ensures (res.Repr - {res}) <= c.Repr
+    ensures fresh(res.Repr - c.Repr)
   {
-    var result := Cast<AsByteConsumer>(c, _ => true);
+    var result := Cast<AsByteConsumer>(c, (casted: AsByteConsumer) => casted.Repr == c.Repr);
     match result {
-      case Some(adaptor) => 
+      case Some(adaptor) =>
+        Axiom(adaptor.Valid());
         res := adaptor.wrapped; 
       case None =>
         res := new AsExternalByteConsumer(c);
@@ -91,13 +115,16 @@ module Consumers {
   }
 
   method FromExternalByteConsumer(c: ExternalByteConsumer) returns (res: ByteConsumer) 
+    requires c.Valid()
     ensures res.Valid()
+    ensures (res.Repr - {res}) <= c.Repr
+    ensures fresh(res.Repr - c.Repr)
   {
-    var result := Cast<AsExternalByteConsumer>(c, _ => true);
+    var result := Cast<AsExternalByteConsumer>(c, (casted: AsExternalByteConsumer) => casted.Repr == c.Repr);
     match result {
       case Some(adaptor) =>
-        adaptor.AssumedValid();
-        res := adaptor.wrapped; 
+        Axiom(adaptor.Valid());
+        res := adaptor.wrapped;
       case None =>
         res := new AsByteConsumer(c);
     }
@@ -107,7 +134,7 @@ module Consumers {
     const bytes: array<uint8>
     var index: int
     var maxIndex: int
-    predicate Valid() reads this {
+    predicate Valid() reads this decreases this, Repr {
       && 0 <= index <= maxIndex <= bytes.Length
       && Repr == {this, bytes}
     }
